Lib.v
@@ -14,6 +14,14 @@ Definition Vec_map {A B C : Type}(f : A -> B -> C) :=
   | ConsV a b lB => ConsV a (f a b) (rec _ lB)
     end.
 
+Fixpoint Vec_map_id {A B : Type}{l : list A}(v : Vec B l) : Vec_map (fun _ x => x) v = v.
+  destruct v.
+  -  reflexivity.
+  -  cbn.
+     f_equal.
+     apply Vec_map_id.
+Defined.
+
 Lemma vec_map_map {A B C D : Type}(f : A -> B -> C) (g : A -> C -> D) {l : list A}
       (v : Vec B l) : Vec_map g (Vec_map f v) = Vec_map (fun a b => g a (f a b)) v.
   induction v; cbn; congruence.
@@ -23,6 +31,12 @@ Definition vec_map_ext {A B C : Type}(f g : A -> B -> C) {l : list A}
       (v : Vec B l) (h : forall a b, f a b = g a b): Vec_map f v = Vec_map g v.
   induction v; cbn; congruence.
 Defined.
+
+Fixpoint vec_max {A : Type}(l : list A) (v : Vec nat l) : nat :=
+  match v with
+    NilV _ => 0
+  | ConsV a b lB => Nat.max b (vec_max lB)
+    end.
 
 Lemma commutes_if {A B : Type}(f : A -> B)(b : bool) x y :
   (if b then f x else f y) = f (if b then x else y).
